define high level state machine

ironfleet/ravana/Service.i.dfy
@@ -1,9 +1,11 @@
 include "Types.i.dfy"
 
 module Service_i {
+  import opened Types_i
+
   predicate Service_Init(s: ServiceState, switches: set<EndPoint>) {
-    s.outstandingCommands == {} &&
-    s.outstandingEvents == {} &&
+    s.outstandingCommands == multiset{} &&
+    s.outstandingEvents == multiset{} &&
     keys_match(s.switchStates, switches)
   }
 
@@ -14,5 +16,62 @@ module Service_i {
   }
 
   predicate Service_NextNewEvent(s: ServiceState, s': ServiceState) {
+    s.switchStates == s'.switchStates &&
+    s.controllerState == s'.controllerState &&
+    s.outstandingCommands == s'.outstandingCommands &&
+    multiset_adds_one(s.outstandingEvents, s'.outstandingEvents)
+  }
+
+  predicate Service_NextApplyEvent(s: ServiceState, s': ServiceState) {
+    s.switchStates == s'.switchStates &&
+    s.outstandingCommands == multiset{} &&
+
+    multiset_adds_one(s'.outstandingEvents, s.outstandingEvents) &&
+    var event := added_obj(s'.outstandingEvents, s.outstandingEvents);
+    var (cs', singleCommands) :=
+        controllerTransition(s.controllerState, event.switch, event.event);
+    s'.controllerState == cs' &&
+    s'.outstandingCommands == seq_to_multiset(singleCommands)
+  }
+
+  predicate Service_NextApplyCommand(s: ServiceState, s': ServiceState) {
+    s.controllerState == s'.controllerState &&
+    s.outstandingCommands == s'.outstandingCommands &&
+
+    multiset_adds_one(s'.outstandingCommands, s.outstandingCommands) &&
+    var command := added_obj(s'.outstandingCommands, s.outstandingCommands);
+
+    command.switch in s.switchStates &&
+    s'.switchStates == s.switchStates[command.switch :=
+        switchTransition(s.switchStates[command.switch], command.command) ]
+  }
+
+  // helpers
+
+  predicate {:opaque} keys_match<A, B>(m: map<A, B>, s: set<A>) {
+    (forall k : A :: k in m ==> k in s) &&
+    (forall k : A :: k in s ==> k in m)
+  }
+
+  predicate multiset_adds_one<A>(m: multiset<A>, m1: multiset<A>) {
+    |m1| == |m| + 1 &&
+    |m1 - m| == 1
+  }
+
+  function {:opaque}
+  added_obj<A>(m: multiset<A>, m1: multiset<A>) : A
+  requires multiset_adds_one<A>(m, m1)
+  {
+    var y :| y in (m1 - m);
+    y
+  }
+
+  function {:opaque} seq_to_multiset<A>(s: seq<A>) : multiset<A>
+  {
+    if s == [] then
+      multiset{}
+    else (
+      seq_to_multiset(s[1..]) + multiset{s[0]}
+    )
   }
 }
